Semantic/CC/Syntax/CaptureSet.lean
@@ -1,0 +1,23 @@
+import Semantic.CC.Debruijn
+namespace CC
+
+inductive Var : Kind -> Sig -> Type where
+| bound : BVar s k -> Var k s
+| free : Nat -> Var k s
+
+inductive CaptureSet : Sig -> Type where
+| empty : CaptureSet s
+| union : CaptureSet s -> CaptureSet s -> CaptureSet s
+| var : Var .var s -> CaptureSet s
+| cvar : Var .cvar s -> CaptureSet s
+
+@[simp]
+instance CaptureSet.instEmptyCollection :
+  EmptyCollection (CaptureSet s) where
+  emptyCollection := CaptureSet.empty
+
+@[simp]
+instance CaptureSet.instUnion : Union (CaptureSet s) where
+  union := CaptureSet.union
+
+end CC
